src/coq/Syntax/ScopeTheory.v
@@ -3,7 +3,7 @@ From Coq Require Import
      List.
 Import ListNotations.
 
-From stdpp Require Import base gmap fin_maps fin_map_dom.
+From stdpp Require Import base gmap fin_maps fin_map_dom ssreflect.
 From Vellvm Require Import
      Numeric.Coqlib
      Utilities
@@ -13,42 +13,17 @@ Set Implicit Arguments.
 Set Strict Implicit.
 (* end hide *)
 
-Lemma app_snoc_app : forall {A} (l l' : list A) x,
-    (l ++ [x]) ++ l' = l ++ (x :: l').
-Proof using.
-  intros.
-  rewrite <- app_assoc; reflexivity.
-Qed.
+(** * Working with stdpp, useful tactics:
+    - solve_proper
+    - solve_map_disjoint
+    - set_solver
+    - simplify_map_eq
+ *)
 
-Section LABELS_THEORY.
-
-  Context {T : Set}.
-
-  Lemma inputs_app: forall (l l' : ocfg T),
-      @inputs T (l ∪ l') = inputs l ∪ inputs l'.
-  Proof using.
-    intros.
-    unfold inputs.
-    (* Is this good style? *)
-    unfold_leibniz.
-    apply dom_union.
-  Qed.
-
-  Lemma outputs_acc_comm:
-    ∀ (i : block_id) (bk : block T) (g : gmap block_id (block T)) (j1 j2 : block_id)
-      (z1 z2 : block T) (y : gset block_id),
-      j1 ≠ j2 →
-      <[i:=bk]> g !! j1 = Some z1 →
-      <[i:=bk]> g !! j2 = Some z2 →
-      outputs_acc j1 z1 (outputs_acc j2 z2 y) = outputs_acc j2 z2 (outputs_acc j1 z1 y).
-  Proof.
-    set_solver.
-  Qed.
-
-  (* TODO: the lib lemma is weirdly specialized, todo ask/PR stdpp *)
+(* TODO: the lib lemma is weirdly specialized, todo ask/PR stdpp *)
 Lemma map_fold_comm_acc
   {K : Type} {M : Type → Type} `{FMap M, ∀ A : Type, Lookup K A (M A), ∀ A : Type, Empty (M A), ∀ A : Type, PartialAlter K A (M A),  OMap M, Merge M, ∀ A : Type, MapFold K A (M A), EqDecision K,
-  FinMap K M}
+                                   FinMap K M}
   {A B} (f : K → A → B → B) (g : B → B) (x : B) (m : M A) :
   (∀ j1 j2 z1 z2 y, f j1 z1 (f j2 z2 y) = f j2 z2 (f j1 z1 y)) →
   (∀ j z y, f j z (g y) = g (f j z y)) →
@@ -57,22 +32,41 @@ Proof.
   intros. apply (map_fold_comm_acc_strong _); [solve_proper|solve_proper|done..].
 Qed.
 
-  Lemma outputs_acc_union_acc : forall (g g' : ocfg T),
+(** * Scope theory: relating elementary graph constructions to scope collections *)
+Section SCOPE_THEORY.
+
+  Context {T : Set}.
+
+(* Preliminaries: [gset_bk_acc/map_fold_bk_acc] *)
+
+  Lemma fold_bk_acc_empty (f : block_id -> block T -> _):
+    fold_bk_acc f ∅ = ∅.
+  Proof.
+    set_solver.
+  Qed.
+
+  Lemma gset_bk_acc_comm : forall f,
+    ∀ (i j : block_id) (bk1 bk2 : block T) (ids : gset block_id),
+      i ≠ j →
+      gset_bk_acc f i bk1 (gset_bk_acc f j bk2 ids) =
+      gset_bk_acc f j bk2 (gset_bk_acc f i bk1 ids).
+  Proof.
+    set_solver.
+  Qed.
+
+  Lemma gset_bk_acc_union_acc : forall f (g g' : ocfg T),
       g ##ₘ g' ->
-      map_fold outputs_acc ∅ (g ∪ g') =
-      map_fold outputs_acc (map_fold outputs_acc ∅ g) g'.
+      map_fold (gset_bk_acc f) ∅ (g ∪ g') =
+      map_fold (gset_bk_acc f) (map_fold (gset_bk_acc f) ∅ g) g'.
   Proof.
     induction g as [|i bk g ? IH] using (map_ind (M := gmap block_id)).
     - intros * _.
-      now rewrite map_empty_union.
-      Undo.
-      now rewrite (left_id ∅ _).
+      by rewrite left_id.
     - intros ? DISJ.
       rewrite <- insert_union_l.
-
       do 2 (rewrite map_fold_insert_L;
-        [| apply outputs_acc_comm |
-           (auto || apply lookup_union_None; now simplify_map_eq)]).
+            [| intros ; eapply gset_bk_acc_comm; eauto |
+              (auto || apply lookup_union_None; by simplify_map_eq)]).
       rewrite IH.
       2: eapply map_disjoint_insert_l; eauto.
       symmetry; apply map_fold_comm_acc.
@@ -80,12 +74,131 @@ Qed.
       intros; set_solver.
   Qed.
 
-  Lemma outputs_acc_union : forall i (b : block T) g g',
-    outputs_acc i b (g ∪ g') = outputs_acc i b g ∪ g'.
+  Lemma fold_bk_acc_union: forall f (g g' : ocfg T),
+      g ##ₘ g' ->
+      fold_bk_acc f (g ∪ g') =
+        fold_bk_acc f g ∪ fold_bk_acc f g'.
+  Proof.
+    induction g as [|i bk g ? IH] using (map_ind (M := gmap block_id)).
+    - intros * _.
+      rewrite fold_bk_acc_empty map_empty_union.
+      set_solver.
+    - intros ? DISJ.
+      rewrite <- insert_union_l.
+      do 2 (rewrite map_fold_insert_L;
+            [| intros; eapply gset_bk_acc_comm; eauto |
+              (auto || apply lookup_union_None; by simplify_map_eq)]).
+      rewrite IH.
+      2: solve_map_disjoint.
+      unfold gset_bk_acc; set_solver.
+  Qed.
+
+  Lemma fold_bk_acc_singleton : forall f i (bk : block T),
+      fold_bk_acc f {[ i := bk]} = f i bk.
+  Proof.
+    intros.
+    rewrite map_fold_singleton.
+    set_solver.
+  Qed.
+
+  Lemma fold_bk_acc_insert: forall f i bk (g : ocfg T),
+      g !! i = None ->
+      fold_bk_acc f (<[ i := bk]> g) = f i bk ∪ fold_bk_acc f g.
+  Proof.
+    intros.
+    rewrite insert_union_singleton_l.
+    rewrite fold_bk_acc_union.
+    by rewrite fold_bk_acc_singleton.
+    solve_map_disjoint.
+  Qed.
+
+  Lemma elem_of_fold_bk_acc :
+    forall f (g : ocfg T) (i : block_id),
+      i ∈ fold_bk_acc f g ->
+      exists j bk, g !! j = Some bk /\ i ∈ f j bk.
+  Proof.
+    induction g as [|i bk g ? IH] using (map_ind (M := gmap block_id)).
+    - intros * IN; rewrite fold_bk_acc_empty in IN; set_solver.
+    - intros j IN.
+      rewrite fold_bk_acc_insert in IN; auto.
+      apply elem_of_union in IN as [IN | IN].
+      + exists i, bk; split; auto.
+        by simplify_map_eq.
+      + apply IH in IN as (k & bkk & LU & IN).
+        do 2 eexists; split; eauto.
+        by simplify_map_eq.
+  Qed.
+
+(* [inputs] *)
+  Lemma inputs_empty :
+    @inputs T ∅ = ∅.
   Proof.
     set_solver.
   Qed.
 
+  Lemma inputs_union: forall (l l' : ocfg T),
+      @inputs T (l ∪ l') = inputs l ∪ inputs l'.
+  Proof.
+    set_solver.
+  Qed.
+
+  Lemma inputs_singleton: forall i (bk : block T),
+      inputs {[ i := bk]} = {[i]}.
+  Proof.
+    intros.
+    unfold inputs.
+    set_solver.
+  Qed.
+
+  Lemma inputs_insert: forall i bk (g : ocfg T),
+      inputs (<[ i := bk]> g) = {[i]} ∪ inputs g.
+  Proof.
+    set_solver.
+  Qed.
+
+  Lemma disjoint_inputs_l (g1 g2 : ocfg T) :
+    g1 ##ₘ g2 ->
+    forall x, x ∈ inputs g2 ->
+         x ∉ inputs g1.
+  Proof.
+    intros * DISJ x; apply map_disjoint_dom in DISJ.
+    set_solver.
+  Qed.
+
+  Lemma disjoint_inputs_r (g1 g2 : ocfg T) :
+    g1 ##ₘ g2 ->
+    forall x, x ∈ inputs g1 ->
+         x ∉ inputs g2.
+  Proof.
+    intros * DISJ x; apply map_disjoint_dom in DISJ.
+    set_solver.
+  Qed.
+
+  Lemma find_block_in_inputs :
+    forall i (g : ocfg T),
+      i ∈ inputs g ->
+      is_Some (g !! i).
+  Proof.
+    intros; by apply elem_of_dom.
+  Qed.
+
+  Lemma free_out_of_inputs :
+    forall i (g : ocfg T),
+      i free in g ->
+      g !! i = None.
+  Proof.
+    intros; by apply not_elem_of_dom.
+  Qed.
+
+  Lemma free_in_cfg_union:
+    forall (g g' : ocfg T) i,
+      i free in (g ∪ g') <->
+      i free in g /\ i free in g'.
+  Proof.
+    set_solver.
+  Qed.
+
+(* [outputs] *)
   Lemma outputs_empty : outputs (T := T) ∅ = ∅.
   Proof.
     set_solver.
@@ -95,143 +208,131 @@ Qed.
       g ##ₘ g' ->
       outputs (g ∪ g') = outputs g ∪ outputs g'.
   Proof.
-    induction g as [|i bk g ? IH] using (map_ind (M := gmap block_id)).
-    - intros * _.
-      rewrite outputs_empty, map_empty_union.
-      set_solver.
-    - intros ? DISJ.
-      rewrite <- insert_union_l.
-      unfold outputs.
-      do 2 (rewrite map_fold_insert_L;
-        [| apply outputs_acc_comm |
-           (auto || apply lookup_union_None; now simplify_map_eq)]).
-      unfold outputs at 1 in IH.
-      rewrite IH.
-      2: solve_map_disjoint.
-      apply outputs_acc_union.
+    apply fold_bk_acc_union.
   Qed.
 
   Lemma outputs_singleton: forall i (bk : block T),
       outputs {[ i := bk]} = successors bk.
   Proof.
-    intros.
-    unfold outputs.
-    rewrite map_fold_singleton.
-    set_solver.
+    apply fold_bk_acc_singleton.
   Qed.
 
   Lemma outputs_insert: forall i bk (g : ocfg T),
       g !! i = None ->
       outputs (<[ i := bk]> g) = successors bk ∪ outputs g.
-  Proof using.
-    intros.
-    rewrite insert_union_singleton_l.
-    rewrite outputs_union.
-    now rewrite outputs_singleton.
-    solve_map_disjoint.
+  Proof.
+    apply fold_bk_acc_insert.
   Qed.
 
-  (* (* TODO: Show symmetric case *) *)
-  (* Lemma wf_ocfg_bid_app_not_in_l : *)
-  (*   forall id (bs bs' : ocfg T), *)
-  (*     In id (inputs bs) -> *)
-  (*     wf_ocfg_bid (bs' ++ bs) -> *)
-  (*     not (In id (inputs bs')). *)
-  (* Proof using. *)
-  (*   intros. destruct bs. *)
-  (*   inversion H. *)
-  (*   inv H. *)
-  (*   apply wf_ocfg_bid_cons_not_in. *)
-  (*   unfold wf_ocfg_bid in *. *)
-  (*   rewrite inputs_app in H0. *)
-  (*   rewrite inputs_cons. rewrite inputs_cons in H0. *)
-  (*   rewrite list_cons_app in H0. *)
-  (*   rewrite app_assoc in H0. *)
-  (*   apply list_norepet_append_left in H0. *)
-  (*   rewrite list_cons_app. *)
-  (*   rewrite list_norepet_app in *. *)
-  (*   intuition. apply list_disjoint_sym. auto. *)
-  (*   unfold wf_ocfg_bid in H0. *)
-  (*   rewrite inputs_app in H0. rewrite inputs_cons in H0. rewrite list_cons_app in H0. *)
-  (*   apply list_norepet_append_commut in H0. rewrite <- app_assoc in H0. *)
-  (*   apply list_norepet_append_right in H0. *)
-  (*   rewrite list_norepet_app in H0. *)
-  (*   destruct H0 as (? & ? & ?). *)
-  (*   red in H2. intro. eapply H2; eauto. *)
-  (* Qed. *)
-
-  (* (* TODO: Show symmetric case *) *)
-  (* Lemma wf_ocfg_app_not_in_r : *)
-  (*   forall id (bs bs' : ocfg T), *)
-  (*     In id (inputs bs) -> *)
-  (*     wf_ocfg_bid (bs' ++ bs) -> *)
-  (*     not (In id (inputs bs')). *)
-  (* Proof using. *)
-  (*   intros. destruct bs. *)
-  (*   inversion H. *)
-  (*   inv H. *)
-  (*   apply wf_ocfg_bid_cons_not_in. *)
-  (*   unfold wf_ocfg_bid in *. *)
-  (*   rewrite inputs_app in H0. *)
-  (*   rewrite inputs_cons. rewrite inputs_cons in H0. *)
-  (*   rewrite list_cons_app in H0. *)
-  (*   rewrite app_assoc in H0. *)
-  (*   apply list_norepet_append_left in H0. *)
-  (*   rewrite list_cons_app. *)
-  (*   rewrite list_norepet_app in *. *)
-  (*   intuition. apply list_disjoint_sym. auto. *)
-  (*   unfold wf_ocfg_bid in H0. *)
-  (*   rewrite inputs_app in H0. rewrite inputs_cons in H0. rewrite list_cons_app in H0. *)
-  (*   apply list_norepet_append_commut in H0. rewrite <- app_assoc in H0. *)
-  (*   apply list_norepet_append_right in H0. *)
-  (*   rewrite list_norepet_app in H0. *)
-  (*   destruct H0 as (? & ? & ?). *)
-  (*   red in H2. intro. eapply H2; eauto. *)
-  (* Qed. *)
-
-  (* Useful tactics:
-    - set_solver
-    - solve_map_disjoint
-    - simplify_map_eq
- *)
-
-  Lemma successors_outputs: forall i b (g : ocfg T),
+  Lemma outputs_elem_of' : forall i b (g : ocfg T),
       g !! i = Some b ->
       successors b ⊆ outputs g.
   Proof.
     intros * Lu.
     rewrite <- (insert_delete _ _ _ Lu).
     rewrite outputs_insert.
-    2: now simplify_map_eq.
+    2: by simplify_map_eq.
     set_solver.
   Qed.
 
-  Lemma successor_outputs: forall i j (b: block T) (g : ocfg T),
-      j ∈ successors b ->
+  Lemma outputs_elem_of : forall i j (b: block T) (g : ocfg T),
       g !! i = Some b ->
+      j ∈ successors b ->
       j ∈ outputs g.
-  Proof using.
-    intros * In Lu.
-    pose proof successors_outputs _ _ Lu.
+  Proof.
+    intros * Lu In.
+    pose proof outputs_elem_of' _ _ Lu.
     set_solver.
   Qed.
 
-  Lemma find_block_in_inputs :
-    forall i (g : ocfg T),
-      i ∈ inputs g ->
-      is_Some (g !! i).
-  Proof using.
-    intros; now apply elem_of_dom.
+  (* predecessors *)
+  Lemma predecessors_empty :
+    forall i,
+      predecessors (T := T) i ∅ = ∅.
+  Proof.
+    unfold predecessors; set_solver.
   Qed.
 
+ Lemma predecessors_union :
+    forall i (g g' : ocfg T),
+      g ##ₘ g' ->
+      predecessors i (g ∪ g') = predecessors i g ∪ predecessors i g'.
+  Proof.
+    intros i; apply fold_bk_acc_union.
+  Qed.
+
+  Lemma predecessors_singleton : forall i j (bk : block T),
+      predecessors j {[ i := bk]} = predecessors_acc j i bk.
+  Proof.
+    intros.
+    unfold predecessors.
+    rewrite map_fold_singleton.
+    set_solver.
+  Qed.
+
+  Lemma predecessors_insert: forall i j bk (g : ocfg T),
+      g !! i = None ->
+      predecessors j (<[ i := bk]> g) = predecessors_acc j i bk ∪ predecessors j g.
+  Proof.
+    intros.
+    rewrite insert_union_singleton_l.
+    rewrite predecessors_union.
+    by rewrite predecessors_singleton.
+    solve_map_disjoint.
+  Qed.
+
+  Lemma predecessors_elem_of :
+    forall (g : ocfg T) (src tgt : block_id) (bk : block T),
+      g !! src = Some bk ->
+      tgt ∈ successors bk ->
+      src ∈ predecessors tgt g.
+  Proof.
+    intros * Lu In.
+    rewrite <- (insert_delete _ _ _ Lu).
+    rewrite predecessors_insert.
+    2: by simplify_map_eq.
+    apply elem_of_union_l.
+    unfold predecessors_acc, is_predecessor.
+    rewrite decide_True; auto.
+    set_solver.
+  Qed.
+
+  Lemma elem_of_predecessors :
+    forall (g : ocfg T) (src tgt : block_id),
+      src ∈ predecessors tgt g ->
+      exists bk, g !! src = Some bk /\ is_predecessor tgt bk = true.
+  Proof.
+    intros * IN.
+    apply elem_of_fold_bk_acc in IN as (j & bk & LU & IN).
+    unfold predecessors_acc in IN.
+    exists bk.
+    destruct (is_predecessor tgt bk); [| set_solver].
+    apply elem_of_singleton in IN; subst; auto.
+  Qed.
+
+  Lemma successor_elem_of :
+    forall (G : ocfg T) (src tgt : block_id) (bk : block T),
+      src ∈ predecessors tgt G ->
+      G !! src = Some bk ->
+      tgt ∈ successors bk.
+  Proof.
+    intros * IN FIND.
+    apply elem_of_predecessors in IN as (bk' & LU & ?).
+    simplify_map_eq.
+    unfold is_predecessor in *.
+    case_match; easy.
+  Qed.
+
+(* [no_reentrance] *)
   Lemma no_reentrance_not_in (g1 g2 : ocfg T) :
     no_reentrance g1 g2 ->
-    forall i, i ∈ outputs g2 -> i ∉ inputs g1.
+    forall i, i ∈ outputs g2 ->
+         i ∉ inputs g1.
   Proof.
     set_solver.
   Qed.
 
-  Lemma no_reentrance_app_l :
+  Lemma no_reentrance_union_l :
     forall (g1 g1' g2 : ocfg T),
       no_reentrance (g1 ∪ g1') g2 <->
       no_reentrance g1 g2 /\ no_reentrance g1' g2.
@@ -239,7 +340,7 @@ Qed.
     set_solver.
   Qed.
 
-  Lemma no_reentrance_app_r :
+  Lemma no_reentrance_union_r :
     forall (g1 g2 g2' : ocfg T),
       g2 ##ₘ g2' ->
       no_reentrance g1 (g2 ∪ g2') <->
@@ -250,554 +351,26 @@ Qed.
     - rewrite outputs_union; set_solver.
   Qed.
 
-  Lemma no_duplicate_bid_not_in_l (g1 g2 : ocfg T) :
-    no_duplicate_bid g1 g2 ->
-    forall x, In x (inputs g2) -> ~ In x (inputs g1).
-  Proof using.
-    intros; eauto using Coqlib.list_disjoint_notin, Coqlib.list_disjoint_sym.
-  Qed.
-
-  Lemma no_duplicate_bid_not_in_r (g1 g2 : ocfg T) :
-    no_duplicate_bid g1 g2 ->
-    forall x, In x (inputs g1) -> ~ In x (inputs g2).
-  Proof using.
-    intros; eauto using Coqlib.list_disjoint_notin, Coqlib.list_disjoint_sym.
-  Qed.
-
   Lemma independent_flows_no_reentrance_l (g1 g2 : ocfg T):
     independent_flows g1 g2 ->
     no_reentrance g1 g2.
-  Proof using.
+  Proof.
     intros INDEP; apply INDEP; auto.
   Qed.
 
   Lemma independent_flows_no_reentrance_r (g1 g2 : ocfg T):
     independent_flows g1 g2 ->
     no_reentrance g2 g1.
-  Proof using.
+  Proof.
     intros INDEP; apply INDEP; auto.
   Qed.
 
-  Lemma independent_flows_no_duplicate_bid (g1 g2 : ocfg T):
+  Lemma independent_flows_disjoint (g1 g2 : ocfg T):
     independent_flows g1 g2 ->
-    no_duplicate_bid g1 g2.
-  Proof using.
+    g1 ##ₘ g2.
+  Proof.
     intros INDEP; apply INDEP; auto.
   Qed.
 
-  Lemma find_block_not_in_inputs:
-    forall bid (l : ocfg T),
-      ~ In bid (inputs l) ->
-      find_block l bid = None.
-  Proof using.
-    induction l as [| bk l IH]; intros NIN; auto.
-    cbn.
-    flatten_goal.
-    - exfalso.
-      flatten_hyp Heq; [| inv Heq].
-      apply NIN.
-      left; rewrite e; reflexivity.
-    - flatten_hyp Heq; [inv Heq |].
-      apply IH.
-      intros abs; apply NIN.
-      right; auto.
-  Qed.
+End SCOPE_THEORY.
 
-  Lemma wf_ocfg_bid_singleton : forall (b : _ T), wf_ocfg_bid [b].
-  Proof using.
-    intros.
-    red.
-    eapply list_norepet_cons; eauto.
-    eapply list_norepet_nil.
-  Qed.
-
-  Lemma wf_ocfg_bid_cons' : forall (b : _ T) (g : ocfg T),
-      not (In (blk_id b) (inputs g)) ->
-      wf_ocfg_bid g ->
-      wf_ocfg_bid (b :: g).
-  Proof using.
-    intros.
-    eapply list_norepet_cons; eauto.
-  Qed.
-
-  Lemma free_in_cfg_cons:
-    forall b (bs : ocfg T) id,
-      free_in_cfg (b::bs) id ->
-      free_in_cfg bs id .
-  Proof using.
-    intros * FR abs; apply FR; cbn.
-    destruct (Eqv.eqv_dec_p (blk_id b) id); [rewrite e; auto | right; auto].
-  Qed.
-
-  Lemma free_in_cfg_app : forall (g1 g2 : ocfg T) b,
-      free_in_cfg (g1 ++ g2) b <->
-      (free_in_cfg g1 b /\ free_in_cfg g2 b).
-  Proof using.
-    intros; split; unfold free_in_cfg; intro FREE.
-    - split; intros abs; eapply FREE; rewrite inputs_app; eauto using in_or_app.
-    - rewrite inputs_app; intros abs; apply in_app_or in abs; destruct FREE as [FREEL FREER]; destruct abs; [eapply FREEL | eapply FREER]; eauto.
-  Qed.
-
-  Lemma wf_ocfg_bid_distinct_labels :
-    forall (g1 g2 : ocfg T) b1 b2,
-      wf_ocfg_bid (g1 ++ g2) ->
-      In b1 (inputs g1) ->
-      In b2 (inputs g2) ->
-      b1 <> b2.
-  Proof using.
-    intros * WF IN1 IN2.
-    eapply wf_ocfg_bid_app_not_in_l in IN2; eauto.
-    destruct (Eqv.eqv_dec_p b1 b2).
-    rewrite e in IN1; contradiction IN2; auto.
-    auto.
-  Qed.
-
-  Lemma predecessors_app :
-    forall (g g' : ocfg T) f,
-      predecessors f (g ++ g') = predecessors f g' ++ predecessors f g.
-  Proof using.
-    induction g' as [| bk g' IH] using rev_ind.
-    - intros; cbn; rewrite !app_nil_r; reflexivity.
-    - intros.
-      unfold predecessors.
-      rewrite app_assoc.
-      rewrite 2 (fold_left_app _ _ [bk]).
-      simpl.
-      break_match_goal.
-      + cbn; f_equal.
-        apply IH.
-      + apply IH.
-  Qed.
-
-  Lemma predecessors_cons :
-    forall (g : ocfg T) bk f,
-      predecessors f (bk :: g) = predecessors f g ++ predecessors f [bk].
-  Proof using.
-    intros.
-    rewrite list_cons_app, predecessors_app.
-    reflexivity.
-  Qed.
-
-  Lemma find_block_In : forall G (bk : block T),
-      find_block G bk.(blk_id) = Some bk ->
-      In bk G.
-  Proof using.
-    induction G as [| x G IH]; intros * FIND; [inv FIND |].
-    cbn in FIND; break_match_hyp; auto.
-    inv FIND; left; reflexivity.
-    right; apply IH; auto.
-  Qed.
-
-  Lemma successor_predecessor :
-    forall (G : ocfg T) (source : block T) target,
-      In target (successors source) ->
-      find_block G source.(blk_id) = Some source ->
-      In source.(blk_id) (predecessors target G).
-  Proof using.
-    intros * IN FIND.
-    apply find_block_In in FIND; revert FIND.
-    induction G as [| bki G IH]; intros * FIND.
-    - inv FIND.
-    - destruct FIND as [EQ | FIND].
-      + subst.
-        clear IH.
-        rewrite predecessors_cons.
-        apply in_or_app; right.
-        cbn.
-        unfold successors in IN.
-        unfold is_predecessor.
-        break_match_goal.
-        left; auto.
-        break_match_hyp; intuition.
-      + rewrite predecessors_cons.
-        apply in_or_app; left.
-        apply IH; auto.
-  Qed.
-
-  Definition predecessors_aux (b : block_id) (G : ocfg T) acc :=
-    fold_left (fun acc bk => if is_predecessor b bk then bk.(blk_id) :: acc else acc) G acc.
-
-  Lemma In_predecessors_is_predecessor_aux :
-    forall (G : ocfg T) acc (src tgt : block_id),
-      In src (predecessors_aux tgt G acc) ->
-      (In src acc \/ exists bk, In bk G /\ src = bk.(blk_id) /\ is_predecessor tgt bk = true).
-  Proof using.
-    intros *; revert acc; induction G as [| bk G IH]; intros acc IN; [left; auto |].
-    cbn in IN.
-    break_match_hyp.
-    - edestruct IH as [INACC | (bk' & INbk & -> & PRED)]; eauto.
-      + destruct INACC as [<- | ?]; [| left; auto].
-        right; exists bk; intuition.
-      + right.
-        exists bk'; intuition.
-    - edestruct IH as [INACC | (bk' & INbk & -> & PRED)]; eauto.
-      right; exists bk'; intuition.
-  Qed.
-
-  Lemma In_predecessors_is_predecessor :
-    forall (G : ocfg T) (src tgt : block_id),
-      In src (predecessors tgt G) ->
-      exists bk, In bk G /\ src = bk.(blk_id) /\ is_predecessor tgt bk = true.
-  Proof using.
-    intros * IN.
-    edestruct In_predecessors_is_predecessor_aux as [INACC | (bk' & INbk & -> & PRED)]; eauto.
-    inv INACC.
-  Qed.
-
-  Lemma find_block_nil:
-    forall b,
-      @find_block T [] b = None.
-  Proof using.
-    reflexivity.
-  Qed.
-
-  Lemma find_block_eq:
-    forall x (b : block T) (bs : ocfg T),
-      blk_id b = x ->
-      find_block (b:: bs) x = Some b.
-  Proof using.
-    intros; cbn.
-    rewrite H.
-    destruct (Eqv.eqv_dec_p x x).
-    reflexivity.
-    contradiction n; reflexivity.
-  Qed.
-
-  Lemma find_block_ineq:
-    forall x (b : block T) (bs : ocfg T),
-      blk_id b <> x ->
-      find_block (b::bs) x = find_block bs x.
-  Proof using.
-    intros; cbn.
-    destruct (Eqv.eqv_dec_p (blk_id b)) as [EQ | INEQ].
-    unfold Eqv.eqv, AstLib.eqv_raw_id in *; intuition.
-    reflexivity.
-  Qed.
-
-  Lemma wf_ocfg_bid_In_is_found :
-    forall (g : ocfg T) bk,
-      wf_ocfg_bid g ->
-      In bk g ->
-      find_block g bk.(blk_id) = Some bk.
-  Proof using.
-    induction g as [| x g IH]; intros * WF IN; [inv IN |].
-    destruct (Eqv.eqv_dec_p x.(blk_id) bk.(blk_id)).
-    - rewrite find_block_eq; auto.
-      destruct IN as [-> | IN]; auto.
-      apply wf_ocfg_bid_cons_not_in in WF.
-      exfalso; apply WF.
-      do 2 red in e; rewrite e.
-      eapply in_map; auto.
-    - rewrite find_block_ineq; [| auto].
-      apply IH.
-      eapply wf_ocfg_bid_cons; eauto.
-      destruct IN; auto.
-      exfalso; subst; eapply n; reflexivity.
-  Qed.
-
-  Lemma predecessor_successor :
-    forall (G : ocfg T) (source target : block_id) (bk : block T),
-      wf_ocfg_bid G ->
-      In source (predecessors target G) ->
-      find_block G source = Some bk ->
-      In target (successors bk).
-  Proof using.
-    intros * WF IN FIND.
-    pose proof In_predecessors_is_predecessor _ _ _ IN as (bk' & IN' & -> & ISPRED).
-    apply wf_ocfg_bid_In_is_found in IN'; auto.
-    rewrite FIND in IN'; inv IN'.
-    unfold is_predecessor in ISPRED.
-    break_match_hyp; intuition.
-  Qed.
-
-  Lemma find_block_app_r_wf :
-    forall (x : block_id) (b : block T) (bs1 bs2 : ocfg T),
-      wf_ocfg_bid (bs1 ++ bs2)  ->
-      find_block bs2 x = Some b ->
-      find_block (bs1 ++ bs2) x = Some b.
-  Proof using.
-    intros x b; induction bs1 as [| hd bs1 IH]; intros * NOREP FIND.
-    - rewrite app_nil_l; auto.
-    - cbn; break_inner_match_goal.
-      + cbn in NOREP; apply wf_ocfg_bid_cons_not_in in NOREP.
-        exfalso; apply NOREP.
-        rewrite e.
-        apply find_some in FIND as [FIND EQ].
-        clear - FIND EQ.
-        rewrite inputs_app; eapply in_or_app; right.
-        break_match; [| intuition].
-        rewrite <- e.
-        eapply in_map; auto.
-      + cbn in NOREP; apply wf_ocfg_bid_cons in NOREP.
-        apply IH; eauto.
-  Qed.
-
-  Lemma find_block_app_l_wf :
-    forall (x : block_id) (b : block T) (bs1 bs2 : ocfg T),
-      wf_ocfg_bid (bs1 ++ bs2)  ->
-      find_block bs1 x = Some b ->
-      find_block (bs1 ++ bs2) x = Some b.
-  Proof using.
-    intros x b; induction bs1 as [| hd bs1 IH]; intros * NOREP FIND.
-    - inv FIND.
-    - cbn in FIND |- *.
-      break_inner_match; auto.
-      apply IH; eauto.
-      eapply wf_ocfg_bid_cons, NOREP.
-  Qed.
-
-  Lemma find_block_tail_wf :
-    forall (x : block_id) (b b' : block T) (bs : ocfg T),
-      wf_ocfg_bid (b :: bs)  ->
-      find_block bs x = Some b' ->
-      find_block (b :: bs) x = Some b'.
-  Proof using.
-    intros.
-    rewrite list_cons_app.
-    apply find_block_app_r_wf; auto.
-  Qed.
-
-  Lemma find_block_free_id :
-    forall (cfg : ocfg T) id,
-      free_in_cfg cfg id ->
-      find_block cfg id = None.
-  Proof using.
-    induction cfg as [| b bs IH]; cbn; intros * FREE; auto.
-    break_inner_match_goal.
-    + exfalso; eapply FREE.
-      cbn; rewrite e; auto.
-    + apply IH.
-      apply free_in_cfg_cons in FREE; auto.
-  Qed.
-
-  Lemma find_block_none_app:
-    forall (g1 g2 : ocfg T) bid,
-      find_block g1 bid = None ->
-      find_block (g1 ++ g2) bid = find_block g2 bid.
-  Proof using.
-    intros; apply find_none_app; auto.
-  Qed.
-
-  Lemma find_block_some_app:
-    forall (g1 g2 : ocfg T) (bk : block T) bid,
-      find_block g1 bid = Some bk ->
-      find_block (g1 ++ g2) bid = Some bk.
-  Proof using.
-    intros; apply find_some_app; auto.
-  Qed.
-
-  Lemma find_block_Some_In_inputs : forall (g : ocfg T) b bk,
-      find_block g b = Some bk ->
-      In b (inputs g).
-  Proof using.
-    induction g as [| hd g IH].
-    - intros * H; inv H.
-    - intros * FIND.
-      destruct (Eqv.eqv_dec_p (blk_id hd) b).
-      cbn; rewrite e; auto.
-      right; eapply IH.
-      erewrite <- find_block_ineq; eauto.
-  Qed.
-
-  Lemma wf_ocfg_bid_find_None_app_l :
-    forall (g1 g2 : ocfg T) b bk,
-      wf_ocfg_bid (g1 ++ g2)%list ->
-      find_block g2 b = Some bk ->
-      find_block g1 b = None.
-  Proof using.
-    induction g1 as [| b g1 IH]; intros * WF FIND.
-    reflexivity.
-    destruct (Eqv.eqv_dec_p (blk_id b) b0).
-    - exfalso.
-      cbn in WF; eapply wf_ocfg_bid_cons_not_in in WF.
-      apply WF.
-      rewrite inputs_app.
-      apply in_or_app; right.
-      rewrite e.
-      apply find_block_Some_In_inputs in FIND; auto.
-    - rewrite find_block_ineq; auto.
-      eapply IH; eauto using wf_ocfg_bid_cons.
-  Qed.
-
-  Lemma find_block_has_id : forall (G : ocfg T) b bk,
-      find_block G b = Some bk ->
-      b = bk.(blk_id).
-  Proof using.
-    induction G as [| bkh G IH].
-    - intros * LU; inv LU.
-    - intros * LU.
-      cbn in LU.
-      break_match_hyp.
-      + inv LU; break_match_hyp; intuition.
-      + apply IH.
-        apply LU.
-  Qed.
-
-  Lemma find_block_map_some :
-    forall (f : block T -> block T) G b bk,
-      (forall bk, blk_id (f bk) = blk_id bk) ->
-      find_block G b = Some bk ->
-      find_block (map f G) b = Some (f bk).
-  Proof using.
-    intros * ID; induction G as [| hd G IH]; intros FIND ; [inv FIND |].
-    cbn in *.
-    rewrite ID.
-    break_match_goal; break_match_hyp; intuition.
-    inv FIND; auto.
-  Qed.
-
-  Lemma find_block_map_none :
-    forall (f : block T -> block T) G b,
-      (forall bk, blk_id (f bk) = blk_id bk) ->
-      find_block G b = None ->
-      find_block (map f G) b = None.
-  Proof using.
-    intros * ID; induction G as [| hd G IH]; intros FIND; [reflexivity |].
-    cbn in *.
-    rewrite ID.
-    break_match_goal; break_match_hyp; intuition.
-    inv FIND; auto.
-  Qed.
-
-  Lemma wf_ocfg_bid_find_block_unique :
-    forall (g : ocfg T) bk1 b1 bk2,
-      wf_ocfg_bid g ->
-      find_block g b1 = Some bk1 ->
-      find_block g b1 = Some bk2 ->
-      bk1 = bk2.
-  Proof using.
-    induction g as [| bk g IH]; intros * WF FIND1 FIND2; [inv FIND1 |].
-    cbn in *.
-    break_match_hyp.
-    inv FIND1; inv FIND2; auto.
-    break_match_hyp; intuition.
-    eapply IH; eauto.
-    eapply wf_ocfg_bid_cons; eauto.
-  Qed.
-
-  Lemma find_block_In' : forall G b (bk : block T),
-      find_block G b = Some bk ->
-      In bk G.
-  Proof using.
-    intros * LU; pose proof find_block_has_id _ _ LU; subst; apply find_block_In; auto.
-  Qed.
-
-  Lemma wf_ocfg_cons_not_in_tail :
-    forall (bk : block T) G,
-      wf_ocfg_bid (bk :: G) ->
-      find_block G bk.(blk_id) = None.
-  Proof using.
-    induction G as [| x G IH]; intros; [reflexivity |].
-    cbn; break_match_goal.
-    - break_match_hyp; intuition.
-      do 2 red in e.
-      exfalso; clear Heqb.
-      red in H.
-      cbn in H.
-      rewrite e in H.
-      inv H.
-      eapply H2; left; reflexivity.
-    - break_match_hyp; intuition.
-      apply IH.
-      apply wf_ocfg_commut_hd in H.
-      eapply wf_ocfg_bid_cons; eauto.
-  Qed.
-
-  Lemma In_find_block :
-    forall (g : ocfg T) bk,
-      In bk g ->
-      exists bk', find_block g bk.(blk_id) = Some bk'.
-  Proof using.
-    induction g as [| x g IH]; intros * IN; [inv IN | ].
-    destruct (Eqv.eqv_dec_p x.(blk_id) bk.(blk_id)).
-    - do 2 red in e; exists x; rewrite find_block_eq; auto.
-    - rewrite find_block_ineq; [| auto].
-      apply IH.
-      destruct IN; auto.
-      exfalso; subst; eapply n; reflexivity.
-  Qed.
-
-  Lemma find_block_map :
-    forall (f : block T -> block T) G b,
-      (forall bk, blk_id (f bk) = blk_id bk) ->
-      find_block (map f G) b = option_map f (find_block G b).
-  Proof using.
-    intros.
-    destruct (find_block G b) eqn:EQ.
-    eapply find_block_map_some in EQ; eauto.
-    eapply find_block_map_none in EQ; eauto.
-  Qed.
-
-End LABELS_THEORY.
-
-Lemma free_in_convert_typ :
-  forall env (bs : list (LLVMAst.block typ)) id,
-    free_in_cfg bs id ->
-    free_in_cfg (convert_typ env bs) id.
-Proof using.
-  induction bs as [| b bs IH]; intros * FR.
-  - red; cbn; auto.
-  - cbn.
-    intros abs.
-    eapply FR.
-    destruct (Eqv.eqv_dec_p (blk_id b) id).
-    left; rewrite e; auto.
-    destruct abs.
-    + cbn in H; unfold Traversal.endo, Traversal.Endo_id in H; cbn in H.
-      exfalso; apply n; rewrite H; reflexivity.
-    + apply IH in H; intuition.
-      eapply free_in_cfg_cons; eauto.
-Qed.
-
-
-
-Section DTyp.
-
-  Lemma convert_typ_terminator_outputs : forall t,
-    terminator_outputs (convert_typ [] t) = terminator_outputs t.
-  Proof using.
-    intros []; cbn; try reflexivity.
-    - induction brs as [| [τ i] brs IH]; cbn; auto.
-      do 2 f_equal.
-      inv IH; auto.
-    - induction brs; cbn; auto; f_equal; auto.
-  Qed.
-
-  Lemma convert_typ_outputs : forall (g : ocfg typ),
-      outputs (convert_typ [] g) = outputs g.
-  Proof using.
-    induction g as [| bk g IH]; [reflexivity |].
-    unfold convert_typ.
-    simpl ConvertTyp_list.
-    rewrite !outputs_cons, <- IH.
-    f_equal.
-    destruct bk; cbn.
-    unfold successors.
-    rewrite <- convert_typ_terminator_outputs.
-    reflexivity.
-  Qed.
-
-  Lemma inputs_convert_typ : forall env bs,
-      inputs (convert_typ env bs) = inputs bs.
-  Proof using.
-    induction bs as [| b bs IH]; cbn; auto.
-    f_equal; auto.
-  Qed.
-
-  Lemma wf_ocfg_bid_convert_typ :
-    forall env (bs : ocfg typ),
-      wf_ocfg_bid bs ->
-      wf_ocfg_bid (convert_typ env bs).
-  Proof using.
-    induction bs as [| b bs IH].
-    - cbn; auto.
-    - intros NOREP.
-      change (wf_ocfg_bid (convert_typ env b :: convert_typ env bs)).
-      apply list_norepet_cons.
-      + apply wf_ocfg_bid_cons_not_in in NOREP.
-        cbn.
-        rewrite inputs_convert_typ; auto.
-      + eapply IH, wf_ocfg_bid_cons; eauto.
-  Qed.
-
-End DTyp.
